\begin{figure}

\begin{itemize}
\item $\LanguageOf{\RegexContext}{\String}=\{\String\}$
\item $\LanguageOf{\RegexContext}{\RegexConcat{\Regex_1}{\Regex_2}} =
\{\StringConcat{\String_1}{\String_2} | \String_1\in\LanguageOf{\RegexContext}{\Regex_1} \wedge \String_2\in\LanguageOf{\RegexContext}{\Regex_2}\}$
\item $\LanguageOf{\RegexContext}{\RegexOr{\Regex_1}{\Regex_2}} =
\{\String | \String\in\LanguageOf{\RegexContext}{\Regex_1} \vee \String\in\LanguageOf{\RegexContext}{\Regex_2}\}$
\item $\LanguageOf{\RegexContext}{\Star{\Regex}} =
\{\String_1\Concat\ldots\Concat\String_n | n\in\Nats \wedge \String_i\in\LanguageOf{\RegexContext}{\Regex}\}$
\item $\LanguageOf{\RegexContext}{\RegexVariable}=\LanguageOf{\RegexContext\setminus(\RegexVariable,\Regex)}{\Regex}$ if, for some unique \Regex{}, $(\RegexVariable,\Regex)\in\RegexContext$.
\item $\LanguageOf{\RegexContext}{\RegexVariable}=\emptyset$
if there does not exist a unique \Regex{} such that $(\RegexVariable,\Regex)\in\RegexContext$

\end{itemize}
%\begin{mathpar}
%\inferrule[Constant Example]
%{
%\String \in \Sigma^*
%}
%{
%\Delta \vdash \String : \String
%}
%
%\inferrule[Userdef Example]
%{
%\Delta' \setminus \{(\Regex,\RegexVariable)\} \vdash \String : \Regex
%}
%{
%\Delta' \cup \{(\Regex,\RegexVariable)\} \vdash \String : \RegexVariable
%}
%
%\inferrule[Concat Example]
%{
%\Delta \vdash \String_1 : \Regex_1\\
%\Delta \vdash \String_2 : \Regex_2\\
%}
%{
%\Delta \vdash \String_1\String_2 : \Regex_1 \Regex_2
%}
%
%\inferrule[Or Example]
%{
%\Delta \vdash \String : \Regex_1\\
%}
%{
%\Delta \vdash \String : \Regex_1 \GBar \Regex_2\\
%}
%
%\inferrule[Empty Star]
%{
%}
%{
%\Delta \vdash \epsilon : \Regex^*
%}
%
%\inferrule[Nonempty Star]
%{
%\Delta \vdash \String_1 : \Regex\\
%\Delta \vdash \String_2 : \Star{\Regex}\\
%}
%{
%\Delta \vdash \String_1\String_2 : \Star{\Regex}
%}
%\end{mathpar}
\caption{Regex Semantics}
\label{fig:regex-semantics}
\end{figure}
