First we will prove some lemmas.

\begin{lemma}
\label{lem:conjunct-builder-rx}
If $\LanguageOf{\SequenceOf{\String_0\SequenceSep\Atom_1\SequenceSep\ldots
\SequenceSep\Atom_n}}=\LanguageOf{\Regex}$
and $\LanguageOf{\AtomAlt}=\LanguageOf{\RegexAlt}$,
then $\LanguageOf{\SequenceOf{\StringAlt\SequenceSep\AtomAlt\SequenceSep
\String_0\SequenceSep\Atom_1\SequenceSep\ldots\SequenceSep\Atom_n}}=
\LanguageOf{\StringAlt\Concat\RegexAlt\Concat\Regex}$.
\end{lemma}
\begin{proof}\leavevmode\\
\begin{tabular}{@{}L@{}L@{}}
\LanguageOf{\SequenceOf{\StringAlt\SequenceSep\AtomAlt\SequenceSep{}
\String_0\SequenceSep\Atom_1\SequenceSep\ldots\SequenceSep\Atom_n}} & = 
\{\StringAlt\Concat\StringAlt'\Concat\String_0\Concat\String_0'\Concat\ldots\Concat\String_n'\Concat\String_n\\
& \hspace{1em} \SuchThat{} \StringAlt'\in\LanguageOf{\AtomAlt}\BooleanAnd{}
\String_i'\in\LanguageOf{\Atom_i}\}\\
& =
\{\StringAlt\Concat\StringAlt'\Concat\String\\
& \hspace{1em} \SuchThat{}
\StringAlt'\in\LanguageOf{\AtomAlt}\BooleanAnd{}
\String\in\LanguageOf{\SequenceOf{\String_0\SequenceSep\Atom_1\SequenceSep\ldots
\SequenceSep\Atom_n}}\\
& =
\{\StringAlt\Concat\StringAlt'\Concat\String\\
& \hspace{1em} \SuchThat{}
\StringAlt\in\LanguageOf{\StringAlt}\BooleanAnd{}
\StringAlt'\in\LanguageOf{\RegexAlt}\BooleanAnd{}
\String\in\LanguageOf{\Regex}\}\\
& =
\LanguageOf{\StringAlt\Concat\RegexAlt\Concat\Regex}
\end{tabular}
\end{proof}

\begin{lemma}
\label{lem:conjunct-rx}
Let $\SequenceOf{\String_0\SequenceSep\Atom_1\SequenceSep
\ldots\Atom_n\SequenceSep\String_n}$ be a conjunct,
and for each $\Atom_i$, there exists a regular expression, $\Regex_i$, such that
$\LanguageOf{\Atom_i}=\Regex_i$.
Then, there exists a regular expression $\Regex$, such that
$\LanguageOf{\SequenceOf{\String_0\SequenceSep\Atom_1\SequenceSep
\ldots\Atom_n\SequenceSep\String_n}}=\LanguageOf{\Regex}$.
\end{lemma}
\begin{proof}
By induction on $n$.

Let $n=0$.
$\Sequence=\SequenceOf{\String_0}$.
Consider the regular expression, $\String_0$.
$\LanguageOf{\String_0}=\{\String_0\}=\LanguageOf{\SequenceOf{\String_0}}$

Let $n>0$,
$\Sequence=\SequenceOf{\String_0\SequenceSep\Atom_1\SequenceSep
\ldots\Atom_n\SequenceSep\String_n}$.
By induction assumption, there exists a regular expression $\Regex'$ such that
$\LanguageOf{\Regex'}=\LanguageOf{\String_1\SequenceSep\Atom_2\ldots
\SequenceSep\Atom_n\String_n}$.
By problem assumption, there exists a regular expression $\Regex_1$ such that
$\LanguageOf{\Atom_1}=\LanguageOf{\Regex_1}$.
Consider $\String_0\Concat\Regex_1\Concat\Regex'$.
By Lemma~\ref{lem:conjunct-builder-rx},
$\LanguageOf{\String_0\Concat\Regex_1\Concat\Regex'}=
\LanguageOf{\SequenceOf{\String_0\SequenceSep\Atom_1\SequenceSep
\ldots\Atom_n\SequenceSep\String_n}}$.
\end{proof}



\begin{lemma}
\label{lem:dnf-builder-rx}
If $\LanguageOf{\DNFOf{\Sequence_2\DNFSep\ldots\DNFSep\Sequence_n}}
=\LanguageOf{\Regex}$
and $\LanguageOf{\Sequence_1}=\LanguageOf{\RegexAlt}$,
then $\LanguageOf{\DNFOf{\Sequence_1\DNFSep\ldots\DNFSep\Sequence_n}}=
\LanguageOf{\RegexOr{\RegexAlt}{\Regex}}$.
\end{lemma}
\begin{proof}\leavevmode\\
\begin{tabular}{@{}L@{}L@{}}
\LanguageOf{\DNFOf{\Sequence_1\ldots\Sequence_n}} & = 
\{\String\SuchThat{} \String\in\LanguageOf{\Sequence_i}
\text{ for some $i\in\RangeIncInc{1}{n}$}\}\\
& =
\{\String\SuchThat{}
\String\in\LanguageOf{\Sequence_1}\BooleanOr{}
\String\in\LanguageOf{\Sequence_i}\\
& \hspace{5em} 
\text{ for some $i\in\RangeIncInc{2}{n}$}\}\\
& =
\{\String\SuchThat{}
\String\in\LanguageOf{\RegexAlt}\BooleanOr{}
\String\in\LanguageOf{\Regex}\}\\
& = \LanguageOf{\RegexOr{\RegexAlt}{\Regex}}\\
\end{tabular}
\end{proof}

\begin{lemma}
\label{lem:dnf-rx}
Let $\DNFOf{\Sequence_1\DNFSep\ldots\SequenceSep\Sequence_n}$ be a dnf regex,
and for each $\Sequence_i$, there exists a regular expression, $\Regex_i$,
such that $\LanguageOf{\Sequence_i}=\Regex_i$.
Then, there exists a regular expression $\Regex$, such that
$\LanguageOf{\DNFOf{\Sequence_1\DNFSep
\ldots\DNFSep\Sequence_n}}=\LanguageOf{\Regex}$.
\end{lemma}
\begin{proof}
By induction on $n$.

Let $n=0$.  Consider $\emptyset$
$\LanguageOf{\DNFOf{}}=\{\}=\LanguageOf{\emptyset}$.

Let $n>0$.
$\DNFRegex=\DNFOf{\Sequence_1\DNFSep\ldots\DNFSep\Sequence_n}$.
By induction assumption, there exists a regular expression $\Regex'$ such that
$\LanguageOf{\Regex'}=
\LanguageOf{\DNFOf{\Sequence_2\DNFSep\ldots\DNFSep\Sequence_n}}$.
By problem assumption, there exists a regular expression $\Regex_1$ such that
$\LanguageOf{\Sequence_1}=\LanguageOf{\Regex_1}$.
Consider $\RegexOr{\Regex_1}{\Regex'}$.
By Lemma~\ref{lem:dnf-builder-rx},
$\LanguageOf{\RegexOr{\Regex_1}{\Regex'}}=
\LanguageOf{\DNFOf{\Sequence_1\DNFSep
\ldots\Sequence_n}}$.
\end{proof}
